@prefix : <https://w3id.org/semanticarts/ontology/gistCore#> .
@prefix msl: <https://w3id.org/semanticarts/ontology/meanSeaLevel#> .
@prefix owl: <http://www.w3.org/2002/07/owl#> .
@prefix rdf: <http://www.w3.org/1999/02/22-rdf-syntax-ns#> .
@prefix xml: <http://www.w3.org/XML/1998/namespace> .
@prefix xsd: <http://www.w3.org/2001/XMLSchema#> .
@prefix gist: <https://w3id.org/semanticarts/ns/ontology/gist/> .
@prefix rdfs: <http://www.w3.org/2000/01/rdf-schema#> .
@prefix skos: <http://www.w3.org/2004/02/skos/core#> .
@base <https://w3id.org/semanticarts/ontology/gistCore#> .

<https://w3id.org/semanticarts/ontology/meanSeaLevel> rdf:type owl:Ontology ;
                                                       owl:imports <https://w3id.org/semanticarts/ontology/gistCore12.1.0> ;
                                                       skos:definition "This is an ontology for mean sea level changes recorded by National Oceanic and Atmospheric Administration (NOAA) stations. It uses the gist upper ontology." ;
                                                       skos:prefLabel "Mean Sea Level" ;
                                                       gist:license "For gist: https://creativecommons.org/licenses/by-sa/3.0/" .

#################################################################
#    Object Properties
#################################################################

###  https://w3id.org/semanticarts/ontology/meanSeaLevel#hasMeanSeaLevelChange
msl:hasMeanSeaLevelChange rdf:type owl:ObjectProperty ;
                          rdfs:range msl:meanSeaLevelChange ;
                          skos:definition "Relates an entity that measured sea level changes to its mean recorded sea level change over some period of time." ;
                          skos:prefLabel "has mean sea level change" .


###  https://w3id.org/semanticarts/ontology/meanSeaLevel#measurementOfSeaLevelRelativeTo
msl:measurementOfSeaLevelRelativeTo rdf:type owl:ObjectProperty ;
                                    rdfs:domain msl:meanSeaLevelChange ;
                                    rdfs:range gist:GeoPoint ;
                                    skos:definition "Relates a mean sea level change to the point on land (benchmark) in relation to which it was a measurement of the sea level change." ;
                                    skos:prefLabel "measurement of sea level relative to" .


#################################################################
#    Data properties
#################################################################

###  https://w3id.org/semanticarts/ontology/meanSeaLevel#StationID
msl:StationID rdf:type owl:DatatypeProperty ;
              rdfs:subPropertyOf gist:idText ;
              rdfs:domain msl:NOAAStation ;
              skos:definition "Relates a NOAA station with its station ID." ;
              skos:prefLabel "station ID" .


###  https://w3id.org/semanticarts/ontology/meanSeaLevel#StationName
msl:StationName rdf:type owl:DatatypeProperty ;
                rdfs:subPropertyOf gist:idText ;
                rdfs:domain msl:NOAAStation ;
                skos:definition "Relates a NOAA station to its name." ;
                skos:prefLabel "station name" .


###  https://w3id.org/semanticarts/ontology/meanSeaLevel#has95PercentConfidenceInterval
msl:has95PercentConfidenceInterval rdf:type owl:DatatypeProperty ;
                                   rdfs:domain gist:Event ;
                                   rdfs:range xsd:double ;
                                   skos:definition "Relates a measurement to its 95% confidence interval, where the unit of measure for the confidence interval is the same as the unit of measure used in the measurement." ;
                                   skos:editorialNote "A 95% confidence interval is a magnitude, with its own numeric value and unit of measure. So to be more explicit, this property relates a measurement to the numeric value of a special 95% confidence interval: the measurement's 95% CI represented with the same unit of measure as the measurement. (In principle, one could use different units to record the confidence interval.)" ;
                                   skos:prefLabel "has 95% confidence interval" .


###  https://w3id.org/semanticarts/ontology/meanSeaLevel#percentageComplete
msl:percentageComplete rdf:type owl:DatatypeProperty ;
                       rdfs:domain gist:Event ;
                       rdfs:range xsd:double ;
                       skos:definition "Relates a multi-year measurement process to the percentage of years within the process in which measurements were taken." ;
                       skos:prefLabel "percentage complete" .


###  https://w3id.org/semanticarts/ontology/meanSeaLevel#yearRange
msl:yearRange rdf:type owl:DatatypeProperty ;
              rdfs:domain gist:Event ;
              rdfs:range xsd:int ;
              skos:definition "Relates an event to the total number of years over which it occurred." ;
              skos:prefLabel "year range" .


#################################################################
#    Classes
#################################################################

###  https://w3id.org/semanticarts/ontology/meanSeaLevel#DistancePerDuration
msl:DistancePerDuration rdf:type owl:Class ;
                        rdfs:subClassOf gist:RatioMagnitude ;
                        skos:definition "Magnitudes for distance changed over a period of time." ;
                        skos:prefLabel "Distance per Duration" .


###  https://w3id.org/semanticarts/ontology/meanSeaLevel#NOAAStation
msl:NOAAStation rdf:type owl:Class ;
                rdfs:subClassOf gist:System ;
                skos:definition "A NOAA (National Oceanic and Atmospheric Administration) station which measures changes in sea level." ;
                skos:prefLabel "NOAA Station" .


###  https://w3id.org/semanticarts/ontology/meanSeaLevel#meanSeaLevelChange
msl:meanSeaLevelChange rdf:type owl:Class ;
                       rdfs:subClassOf gist:HistoricalEvent ;
                       skos:definition "The mean sea level change, relative to a fixed point on land, recorded over a period of time by some entity." ;
                       skos:prefLabel "Mean Sea Level Change" .


#################################################################
#    Individuals
#################################################################

###  https://w3id.org/semanticarts/ontology/meanSeaLevel#_century
msl:_century rdf:type owl:NamedIndividual ,
                      gist:DurationUnit ;
             gist:hasBaseUnit gist:_second ;
             gist:conversionFactor "3.1556952E9"^^xsd:double ;
             gist:symbol "C" ;
             skos:definition "A unit of measure corresponding to 100 years." ;
             skos:prefLabel "century" .


###  https://w3id.org/semanticarts/ontology/meanSeaLevel#_feetPerCentury
msl:_feetPerCentury rdf:type owl:NamedIndividual ,
                             gist:RatioUnit ;
                    gist:hasDenominator msl:_century ;
                    gist:hasNumerator msl:_foot ;
                    gist:symbol "ft/C" ;
                    skos:definition "A ratio unit. A measure for change in feet per century." ;
                    skos:prefLabel "feet per century" .


###  https://w3id.org/semanticarts/ontology/meanSeaLevel#_foot
msl:_foot rdf:type owl:NamedIndividual ,
                   gist:DistanceUnit ;
          gist:hasBaseUnit gist:_meter ;
          gist:conversionFactor "0.3048"^^xsd:double ;
          gist:symbol "ft" ;
          skos:definition "A unit of measure in the Imperial system corresponding to a little less than a third of a meter. (The precise conversion factor is given as a datatype property.)" ;
          skos:prefLabel "foot" .


###  https://w3id.org/semanticarts/ontology/meanSeaLevel#_millimeter
msl:_millimeter rdf:type owl:NamedIndividual ,
                         gist:DistanceUnit ;
                gist:hasBaseUnit gist:_meter ;
                gist:conversionFactor "0.001"^^xsd:double ;
                gist:symbol "mm" ;
                skos:definition "A unit of measure for one thousandth of a meter." ;
                skos:prefLabel "millimeter" .


###  https://w3id.org/semanticarts/ontology/meanSeaLevel#_millimetersPerYear
msl:_millimetersPerYear rdf:type owl:NamedIndividual ,
                                 gist:RatioUnit ;
                        gist:hasDenominator msl:_year ;
                        gist:hasNumerator msl:_millimeter ;
                        gist:symbol "mm/yr" ;
                        skos:definition "A ratio unit. A measure for change in millimeters per year." ;
                        skos:prefLabel "millimeters per year" .


###  https://w3id.org/semanticarts/ontology/meanSeaLevel#_year
msl:_year rdf:type owl:NamedIndividual ,
                   gist:DurationUnit ;
          gist:hasBaseUnit gist:_second ;
          gist:conversionFactor "3.1536E7"^^xsd:double ;
          gist:symbol "yr" ;
          skos:definition "A unit of measure for 365 days." ;
          skos:prefLabel "year" .


###  Generated by the OWL API (version 4.5.26.2023-07-17T20:34:13Z) https://github.com/owlcs/owlapi
